\documentclass[11pt]{exam}

\input{../common.tex}
\begin{document}
\customheading{\today}{Direct Proofs: P5b Subset System}{Fall 2024}{CS 30 - Discrete Maths}

\section*{}
\begin{parts}
    \part For any $j \geq 1$ and any $k \in \N$, argue that
        \begin{enumerate}
            \item if $F(j-1, k) = 1$ then $F(j, k) = 1$
            \begin{customsolutionbox}

                To prove this, let's consider the following:
                \begin{gather}
                    \text{let's fix } S \subseteq \{1, 2, 3, \ldots j\} \\
                \end{gather}
                Suppose $j \not \in S$, we have a subset of $S^{*} = S \setminus \{j\} = \{1, 2, \ldots, j-1\}$,such that $\sum_{i \in S^{*}} a_{i} = k$. Therefore, since $S^{*} \subseteq S$, we conclude that $\sum_{i \in S} a_{i} = k$ hence $F(j, k) = 1$
            \end{customsolutionbox}

            \item if $F(j-1, k-a_{j}) = 1$ then $F(j, k) = 1$
            \begin{customsolutionbox}
                To prove this, let's consider the following:
                \begin{gather}
                    \text{let's fix } S \subseteq \{1, 2, 3, \ldots j\} \\
                \end{gather}
                Suppose $j \in S$ such that $\sum_{i \in S} a_{i} = k$ and $F(j, k) = 1$, there exists a subset $S^{*} = S \setminus \{j\} = \{1, 2, \ldots, j-1\}$ such that $\sum_{i \in S^{*}} a_{i} = k - a_j$ hence the assumption $F(j-1, k-a_j) = 1$ is true, and overall the implication is true.
            \end{customsolutionbox}
        \end{enumerate}

    \part For any $j \geq 1$ and any $k \in \N$ argue that $F(j, k) = 1$ then either $F(j-1, k) = 1$ or $F(j-1, k-a_{j}) = 1$
        \begin{customsolutionbox}

            To prove that $F(j-1, k) = 1$ or $F(j-1, k-a_{j}) = 1$, consider the following:
            \begin{gather}
                \text{let's fix } S \subseteq \{1, 2, 3, \ldots j\} \\
            \end{gather}
            \begin{enumerate}
                \item Case 1: $j \not \in S$ and $F(j, k) = 1$. In this case, the assumption is that there exists a subset $S^{*} = S \setminus \{j\} = \{1, 2, \ldots, j-1\}$ such that $\sum_{i \in S^{*}} a_{i} = k$. Therefore, we can conclude that $F(j-1, k) = 1$.
                \item Case 2. $j \in S$. In this case, we assume there exists a subset of $S$ such that $\sum_{i \in S} a_{i} = k$ hence $F(j, k) = 1$. We can conclude there is a subset $S^{*} = S \setminus \{j\} = \{1, 2, \ldots, j-1\}$ such that $\sum_{i \in S^{*}} a_i = k - a_j$ hence  $F(j-1, k-a_j) = 1$
            \end{enumerate}
            Thus, we have shown that if $F(j-1, k) = 1$ or $F(j-1, k-a_j) = 1$ then it follows that $F(j,k) = 1$
        \end{customsolutionbox}
\end{parts}
\end{document}