\documentclass[11pt]{exam}

\input{../common.tex}
\begin{document}
\customheading{\today}{Direct Proofs: P5b Subset System}{Fall 2024}{CS 30 - Discrete Maths}

\section*{}
\begin{parts}
    \part For any $j \geq 1$ and any $k \in \N$, argue that
        \begin{enumerate}
            \item if $F(j-1, k) = 1$ then $F(j, k) = 1$
            \begin{customsolutionbox}
                This implies that if there exists a subset $S' \subseteq \{1, 2, 3, \ldots j-1\}$ such that $\sum_{i \in S'} a_{i} = k$, then there exists a subset of $S \subseteq \{1, 2, 3, \ldots j\}$ such that $F(j, k) = 1$ \\

                To prove this, let's consider the following:
                \begin{gather}
                    \text{let} \hs S \subseteq \{1, 2, \ldots, j\} \\
                    \text{and let } S' \subseteq \{1, 2, \ldots, j-1\}
                \end{gather}
                \begin{itemize}
                    \item Case 1: if $j \not \in S$, then we can consider a subset $S' \subseteq S$ such that $\sum_{i \in S'} a_{i} = k$. This aligns with our assumption that $F(j-1, k) =1$
                    \item Case 2: if $j \in S$ then we consider the subsets of $S$. In this case, \textit{there exists} a subset $S' \subseteq S$ such that $\sum_{i \in S'} a_{i} = k$. Thus, it follows that $F(j, k) = 1$.
                \end{itemize}
            \end{customsolutionbox}

            \item if $F(j-1, k-a_{j}) = 1$ then $F(j, k) = 1$
            \begin{customsolutionbox}
                This implies that if there exists a subset $S' \subseteq S$, where $S = \{1, 2, \ldots, j\}$, such that $\sum_{i \in S'} a_{i} = k-a_{j}$, then it follows that $F(j, k) = 1$ \\

                To prove this consider the following:
                \begin{gather}
                    \text{let} \hs S \subseteq \{1, 2, \ldots, j\} \\
                \end{gather}
                \begin{enumerate}
                    \item Case 1: Suppose $j \not \in S$. If there exists a subset $S' \subseteq S$ such that $\sum_{i \in S'} a_{i} = k - a_{j}$, then it follows that $F(j-1, k-a_{j}) = 1$. Here the assumption is that $k$ is the sum of first $j$ elements.
                    \item Case 2: Suppose $j \in S$. If there exists a subset $S' \subseteq S$ such that $\sum_{i \in S'} a_{i}= k-a_{j}$, then adding $a_{j}$ gives $\sum_{i \in S'} a_{i} +a_{j} =k$. Therefore, it follows that $F(j, k) = 1$.
                \end{enumerate}
            \end{customsolutionbox}
        \end{enumerate}

    \part For any $j \geq 1$ and any $k \in \N$ argue that $F(j, k) = 1$ then either $F(j-1, k) = 1$ or $F(j-1, k-a_{j}) = 1$
        \begin{customsolutionbox}
            $F(j, k) =1$, implies that there exists subset of $S$, where $S \subseteq \{1, 2, \ldots, j\}$, such that $\sum_{i \in S'} a_{i} = k$. here $S' \subseteq S$ \\

            To prove if $F(j-1, k) = 1$ or $F(j-1, k-a_{j}) = 1$, consider the following:
            \begin{gather}
                \text{let} \hs S \subseteq \{1, 2, \ldots, j\} \\
            \end{gather}
            \begin{enumerate}
                \item If $F(j, k)= 1$ and $j \not \in S$, then $S \subseteq \{1, 2, \ldots j-1\}$. If there exists $S' \subseteq S$ such that $\sum_{i \in S'} a_{i} = k$ then this implies that $F(j-1, k) =1$.

                \item If $F(j, k)= 1$ and $j \in S$, then $S \subseteq \{1, 2, \ldots j\}$. If there exists $S' \subseteq S$ such that $\sum_{i \in S'} a_{i}= k- a_{j}$ then this implies $F(j-1, k-a_{j}) =1$.
            \end{enumerate}

            Conclusion: Both cases are valid because there exists a subset $S$ that satisfies the conditions.
        \end{customsolutionbox}
\end{parts}
\end{document}